theories/heap_lang/lib/lock.v
@@ -6,72 +6,63 @@ Import uPred.
 (** * Lock interface *)
 
 (** Operations *)
-Class LockImpl : Set := {
-  newlock' : val; acquire : val; release : val
-}.
-Arguments newlock' _ : clear implicits.
-Arguments acquire _ : clear implicits.
-Arguments release _ : clear implicits.
+Class LockImpl : Set := { newlock' : val; acquire : val; release : val }.
 
-Structure lock Σ `{heapG Σ} {LI : LockImpl} := Lock {
+Structure lock `{heapG Σ} {LI : LockImpl} := Lock {
   (** Predicates. Name ties [locked] to [is_lock]. *)
   name : Type;
-  is_lock (N: namespace) (γ: name) (lock: val) (R: iProp Σ) : iProp Σ;
+  is_lock (γ: name) (lock: val) (R : iProp Σ) : iProp Σ;
   locked (γ: name) : iProp Σ;
   (** Structure *)
-  is_lock_ne N γ lk n: Proper (dist n ==> dist n) (is_lock N γ lk);
-  is_lock_persistent N γ lk R : PersistentP (is_lock N γ lk R);
+  is_lock_ne γ lk n: Proper (dist n ==> dist n) (is_lock γ lk);
+  is_lock_persistent γ lk R : PersistentP (is_lock γ lk R);
   locked_timeless γ : TimelessP (locked γ);
   locked_exclusive γ : locked γ -∗ locked γ -∗ False;
   (** Operations *)
   newlock'_spec p N (R : iProp Σ) :
     heapN ⊥ N →
-    {{{ heap_ctx }}} newlock' LI () @ p; ⊤
-    {{{ lk γ, RET lk;  is_lock N γ lk R ∗ locked γ }}};
-  acquire_spec p N γ lk R :
-    {{{ is_lock N γ lk R }}} acquire LI lk @ p; ⊤ {{{ RET (); locked γ ∗ R }}};
-  release_spec p N γ lk R :
-    {{{ is_lock N γ lk R ∗ locked γ ∗ R }}} release LI lk @ p; ⊤ {{{ RET (); True }}}
+    {{{ heap_ctx }}} newlock' () @ p; ⊤
+    {{{ lk γ, RET lk;  is_lock γ lk R ∗ locked γ }}};
+  acquire_spec p γ lk R :
+    {{{ is_lock γ lk R }}} acquire lk @ p; ⊤ {{{ RET (); locked γ ∗ R }}};
+  release_spec p γ lk R :
+    {{{ is_lock γ lk R ∗ locked γ ∗ R }}} release lk @ p; ⊤ {{{ RET (); True }}}
 }.
-
-Arguments name {_ _ _} _.
-Arguments is_lock {_ _ _} _  _ _ _ _.
-Arguments locked {_ _ _} _  _.
+Arguments lock _ {_ _}.
 
 Existing Instances is_lock_ne is_lock_persistent locked_timeless.
 
-Instance is_lock_proper Σ `{heapG Σ, LockImpl} (L : lock Σ) N lk R:
-  Proper ((≡) ==> (≡)) (is_lock L N lk R) := ne_proper _.
+Instance is_lock_proper `{heapG Σ, LI : LockImpl} (L : lock Σ) lk R:
+  Proper ((≡) ==> (≡)) (is_lock L lk R) := ne_proper _.
 
 (** * Initially unlocked locks *)
-Definition newlock (LI : LockImpl) : val := λ: <>,
-  let: "lk" := newlock' LI () in release LI "lk" ;; "lk".
+Definition newlock {LI : LockImpl} : val := λ: <>,
+  let: "lk" := newlock' () in release "lk" ;; "lk".
 
 Section newlock.
   Context `{heapG Σ, LI : LockImpl} (L : lock Σ).
 
   Lemma newlock_spec p N (R : iProp Σ) :
     heapN ⊥ N →
-    {{{ heap_ctx ∗ R }}} newlock LI () @ p; ⊤
-    {{{ lk γ, RET lk; is_lock L N γ lk R }}}.
+    {{{ heap_ctx ∗ R }}} newlock () @ p; ⊤
+    {{{ lk γ, RET lk; is_lock L γ lk R }}}.
   Proof.
-    iIntros (? Φ) "[#Hh Hr] HΦ"; wp_lam.
-    wp_bind (newlock' _ _); iApply (newlock'_spec _ _ _ _ R with "[$Hh]");
-      first done; iNext; iIntros (lk γ) "[#Hlk Hl]"; wp_let.
-    wp_bind (release _ _); iApply (release_spec with "[$Hlk $Hl $Hr]"); iNext;
-      iIntros "_"; wp_seq.
+    iIntros (? Φ) "[#Hh Hr] HΦ". wp_lam.
+    wp_apply (newlock'_spec L _ _ R with "[$Hh]"); first done.
+      iIntros (lk γ) "[#Hlk Hl]". wp_let.
+    wp_apply (release_spec with "[$Hlk $Hl $Hr]"). iIntros "_". wp_seq.
     by iApply ("HΦ" with "[$Hlk]").
   Qed.
 End newlock.
 
 (** * Synchronization *)
 Section sync_code.
-  Context (LI : LockImpl).
+  Context {LI : LockImpl}.
 
   Definition sync_with : val := λ: "lk" "f",
-    acquire LI "lk" ;; let: "r" := "f" () in release LI "lk" ;; "r".
+    acquire "lk" ;; let: "r" := "f" () in release "lk" ;; "r".
   Definition make_sync : val := λ: <>,
-    let: "lk" := newlock LI () in sync_with "lk".
+    let: "lk" := newlock () in sync_with "lk".
 End sync_code.
 
 Section sync_proof.
@@ -89,28 +80,27 @@ Section sync_proof.
   Global Instance is_sync_ne n v : Proper (dist n ==> dist n) (is_sync v).
   Proof. solve_proper. Qed.
 
-  Lemma sync_with_spec p N γ lk (R : iProp Σ) :
-    {{{ is_lock L N γ lk R }}} sync_with LI lk @ p; ⊤
+  Lemma sync_with_spec p γ lk (R : iProp Σ) :
+    {{{ is_lock L γ lk R }}} sync_with lk @ p; ⊤
     {{{ sync, RET sync; is_sync sync R }}}.
   Proof.
     iIntros (Φ) "#Hlk HΦ". wp_lam.
     iApply "HΦ". iAlways. iIntros (p' e ψ) "% He". wp_let.
-    wp_bind (acquire _ _). iApply (acquire_spec with "Hlk"). iNext.
+    wp_apply (acquire_spec with "Hlk").
       iIntros "[Hlocked Hr]". wp_seq. wp_let.
-    iApply ("He" with "[$Hr]"). iNext. iIntros (v) "Hr HΨ". wp_let.
-    wp_bind (release _ _). iApply (release_spec with "[$Hlk $Hlocked $Hr]").
-      iNext. rewrite wand_True. wp_seq. iExact "HΨ".
+    wp_apply ("He" with "[$Hr]"). iIntros (v) "Hr HΨ". wp_let.
+    wp_apply (release_spec with "[$Hlk $Hlocked $Hr]"). iIntros "_".
+      wp_seq. iExact "HΨ".
   Qed.
 
   Lemma make_sync_spec p N (R : iProp Σ) :
     heapN ⊥ N →
-    {{{ heap_ctx ∗ R }}} make_sync LI () @ p; ⊤
+    {{{ heap_ctx ∗ R }}} make_sync () @ p; ⊤
     {{{ sync, RET sync; is_sync sync R }}}.
   Proof.
-    iIntros (? Φ) "[#Hh HR] HΦ"; wp_lam.
-    wp_bind (newlock _ _).
-      iApply (newlock_spec _ _ _ R with "[$Hh $HR]"); first done.
-      iNext. iIntros (lk γ) "#Hlk". wp_let.
+    iIntros (? Φ) "[#Hh HR] HΦ". wp_lam.
+    wp_apply (newlock_spec L _ _ R with "[$Hh $HR]"); first done.
+      iIntros (lk γ) "Hlk". wp_let.
     by iApply (sync_with_spec with "[$Hlk] [$HΦ]").
   Qed.
 End sync_proof.
